Algebra_Ex/Coset.thy
@@ -1,0 +1,157 @@
+(* Normal subgroup, quotient group, following HOL/Algebra/Coset. *)
+
+theory Coset
+imports Group
+begin
+
+subsection \<open>Cosets\<close>
+
+definition r_coset :: "_ \<Rightarrow> 'a set \<Rightarrow> 'a \<Rightarrow> 'a set" (infixl "#>\<index>" 60) where
+  "H #>\<^bsub>G\<^esub> a = (\<Union>h\<in>H. {h \<otimes>\<^bsub>G\<^esub> a})"
+setup {* add_rewrite_rule @{thm r_coset_def} *}
+
+definition RCOSETS  :: "_ \<Rightarrow> 'a set \<Rightarrow> ('a set) set" ("rcosets\<index> _" [81] 80) where
+  "rcosets\<^bsub>G\<^esub> H = (\<Union>a\<in>carrier G. {H #>\<^bsub>G\<^esub> a})"
+setup {* add_rewrite_rule @{thm RCOSETS_def} *}
+
+theorem is_rcoset: fixes G (structure) shows
+  "s \<in> rcosets H \<Longrightarrow> \<exists>a\<in>carrier G. s = H #> a" by auto2
+setup {* add_forward_prfstep_cond @{thm is_rcoset} [with_cond "?s \<noteq> \<one>\<^bsub>?G'\<^esub>"] *}
+
+theorem r_coset_bij [rewrite_back]: fixes G (structure) shows
+  "group G \<Longrightarrow> elt a \<Longrightarrow> subset H \<Longrightarrow> card H = card (H #> a)"
+  by (tactic {* auto2s_tac @{context}
+    (CHOOSE "f, \<forall>h. f h = h \<otimes> a" THEN
+     OBTAIN "bij_betw f H (H #> a)" WITH
+     (OBTAIN "inj_on f H" THEN
+      OBTAIN "\<forall>y\<in>(H #> a). \<exists>x\<in>H. f x = y" WITH CHOOSE "x\<in>H, y = x \<otimes> a")) *})
+
+theorem r_coset_eqI [backward1]: fixes G (structure) shows
+  "is_subgroup H G \<Longrightarrow> elt a \<Longrightarrow> elt b \<Longrightarrow> a \<otimes> inv b \<in> H \<Longrightarrow> H #> a = H #> b"
+  by (tactic {* auto2s_tac @{context}
+    (OBTAIN "b \<otimes> inv a \<in> H" WITH OBTAIN "inv (a \<otimes> inv b) = b \<otimes> inv a" THEN
+     OBTAIN "\<forall>x. x \<in> (H #> a) \<longleftrightarrow> x \<in> H #> b" WITH
+      (CASE "x \<in> H #> a" WITH
+        (CHOOSE "h \<in> H, x = h \<otimes> a" THEN OBTAIN "x = h \<otimes> a \<otimes> inv b \<otimes> b") THEN
+       CASE "x \<in> H #> b" WITH
+        (CHOOSE "h \<in> H, x = h \<otimes> b" THEN OBTAIN "x = h \<otimes> b \<otimes> inv a \<otimes> a"))) *})
+
+theorem r_coset_disjoint [backward1]: fixes G (structure) shows
+  "elt a \<Longrightarrow> elt b \<Longrightarrow> is_subgroup H G \<Longrightarrow> H #> a \<noteq> H #> b \<Longrightarrow> (H #> a) \<inter> (H #> b) = {}"
+  by (tactic {* auto2s_tac @{context}
+    (CHOOSE "x, x \<in> (H #> a) \<inter> (H #> b)" THEN
+     CHOOSES ["ha\<in>H, x = ha \<otimes> a", "hb\<in>H, x = hb \<otimes> b"] THEN
+     OBTAIN "a \<otimes> inv b = inv ha \<otimes> hb") *})
+
+theorem r_cosets_union_G [rewrite]: fixes G (structure) shows
+  "is_subgroup H G \<Longrightarrow> \<Union>(rcosets H) = carrier G"
+  by (tactic {* auto2s_tac @{context}
+    (OBTAIN "carrier G \<subseteq> \<Union>(rcosets H)" WITH
+      (OBTAIN "\<forall>a\<in>carrier G. a \<in> H #> a" WITH OBTAIN "a = \<one> \<otimes> a")) *})
+
+theorem lagrange: fixes G (structure) shows
+  "finite (carrier G) \<Longrightarrow> is_subgroup H G \<Longrightarrow> card (rcosets H) * card H = order G"
+  by (tactic {* auto2s_tac @{context}
+    (OBTAIN "\<forall>S T. S \<in> rcosets H \<longrightarrow> T \<in> rcosets H \<longrightarrow> S \<noteq> T \<longrightarrow> S \<inter> T = {}" THEN
+     OBTAIN "carrier G = \<Union>(rcosets H)") *})
+
+definition set_mult :: "_ \<Rightarrow> 'a set \<Rightarrow> 'a set \<Rightarrow> 'a set" (infixl "<#>\<index>" 60) where
+  "H <#>\<^bsub>G\<^esub> K = (\<Union>h\<in>H. \<Union>k\<in>K. {h \<otimes> \<^bsub>G\<^esub> k})"
+setup {* add_rewrite_rule @{thm set_mult_def} *}
+theorem set_multI [backward]: "h \<in> H \<Longrightarrow> k \<in> K \<Longrightarrow> h \<otimes>\<^bsub>G\<^esub> k \<in> H <#>\<^bsub>G\<^esub> K" by auto2
+
+definition is_normal_subgroup :: "'a set \<Rightarrow> ('a, 'b) monoid_scheme \<Rightarrow> bool" where
+  "is_normal_subgroup H G \<longleftrightarrow>
+    is_subgroup H G \<and>
+    (\<forall>a h. elt\<^bsub>G\<^esub> a \<longrightarrow> h \<in> H \<longrightarrow> a \<otimes>\<^bsub>G\<^esub> h \<otimes>\<^bsub>G\<^esub> inv\<^bsub>G\<^esub> a \<in> H)"
+setup {* add_backward_prfstep (equiv_backward_th @{thm is_normal_subgroup_def}) *}
+
+lemma is_normal_subgroupD: fixes G (structure) shows
+  "is_normal_subgroup H G \<Longrightarrow> is_subgroup H G"
+  "is_normal_subgroup H G \<Longrightarrow> elt a \<Longrightarrow> h \<in> H \<Longrightarrow> a \<otimes> h \<otimes> inv a \<in> H"
+  by (simp add: is_normal_subgroup_def)+
+setup {* add_forward_prfstep @{thm is_normal_subgroupD(1)} *}
+setup {* add_backward2_prfstep @{thm is_normal_subgroupD(2)} *}
+
+lemma is_normal_subgroupD' [backward2]: fixes G (structure) shows
+  "elt a \<Longrightarrow> is_normal_subgroup H G \<Longrightarrow> h \<in> H \<Longrightarrow> inv a \<otimes> h \<otimes> a \<in> H"
+  by (tactic {* auto2s_tac @{context} (OBTAIN "a = inv (inv a)") *})
+
+theorem set_mult_normal_cosets [rewrite]: fixes G (structure) shows
+  "elt a \<Longrightarrow> elt b \<Longrightarrow> is_normal_subgroup H G \<Longrightarrow> (H #> a) <#> (H #> b) = H #> (a \<otimes> b)"
+  by (tactic {* auto2s_tac @{context}
+    (OBTAIN "\<forall>x. x \<in> (H #> a) <#> (H #> b) \<longleftrightarrow> x \<in> H #> (a \<otimes> b)" WITH
+      (CASE "x \<in> (H #> a) <#> (H #> b)" WITH
+        (CHOOSE "x1 \<in> H #> a, x2 \<in> H #> b, x = x1 \<otimes> x2" THEN
+         CHOOSE "h1 \<in> H, x1 = h1 \<otimes> a" THEN CHOOSE "h2 \<in> H, x2 = h2 \<otimes> b" THEN
+         OBTAIN "x = (h1 \<otimes> a) \<otimes> (h2 \<otimes> inv a \<otimes> a \<otimes> b)" THEN
+         OBTAIN "a \<otimes> h2 \<otimes> inv a \<in> H") THEN
+       CASE "x \<in> H #> (a \<otimes> b)" WITH
+        (CHOOSE "h \<in> H, x = h \<otimes> (a \<otimes> b)" THEN OBTAIN "x = (h \<otimes> a) \<otimes> (\<one> \<otimes> b)"))) *})
+
+definition FactGroup :: "_ \<Rightarrow> 'a set \<Rightarrow> ('a set) monoid" (infixl "Mod" 65) where
+  "FactGroup G H = \<lparr>carrier = rcosets\<^bsub>G\<^esub> H, mult = set_mult G, one = H #>\<^bsub>G\<^esub> \<one>\<^bsub>G\<^esub>\<rparr>"
+
+lemma FactGroup_sel:
+  "elt\<^bsub>G Mod H\<^esub> x \<longleftrightarrow> x \<in> rcosets\<^bsub>G\<^esub>H"
+  "\<one>\<^bsub>(G Mod H)\<^esub> = H #>\<^bsub>G\<^esub> \<one>\<^bsub>G\<^esub>"
+  "S \<otimes>\<^bsub>(G Mod H)\<^esub> T = S <#>\<^bsub>G\<^esub> T" by (simp add: FactGroup_def struct_elt_def)+
+setup {* add_forward_prfstep_cond (equiv_forward_th @{thm FactGroup_sel(1)}) [with_term "?x", with_term "?G Mod ?H"] *}
+setup {* add_forward_prfstep_cond (equiv_backward_th @{thm FactGroup_sel(1)}) [with_term "?G Mod ?H"] *}
+setup {* add_backward_prfstep (equiv_forward_th @{thm FactGroup_sel(1)}) *}
+setup {* add_backward_prfstep (equiv_backward_th @{thm FactGroup_sel(1)}) *}
+setup {* fold add_rewrite_rule @{thms FactGroup_sel(2,3)} *}
+
+theorem FactGroup_is_group: fixes G (structure) shows
+  "is_normal_subgroup H G \<Longrightarrow> group (G Mod H)"
+  by (tactic {* auto2s_tac @{context}
+    (OBTAIN "monoid (G Mod H)" THEN
+     OBTAIN "\<forall>S. elt\<^bsub>G Mod H\<^esub> S \<longrightarrow> (\<exists>T. elt\<^bsub>G Mod H\<^esub> T \<and> T \<otimes>\<^bsub>G Mod H\<^esub> S = \<one>\<^bsub>G Mod H\<^esub>)" WITH
+      (CHOOSE "x, elt\<^bsub>G\<^esub> x \<and> S = H #> x" THEN
+       OBTAIN "(H #> inv x) \<otimes>\<^bsub>G Mod H\<^esub> (H #> x) = \<one>\<^bsub>G Mod H\<^esub>")) *})
+
+definition kernel :: "('a, 'm) monoid_scheme \<Rightarrow> ('b, 'n) monoid_scheme \<Rightarrow>  ('a \<Rightarrow> 'b) \<Rightarrow> 'a set" where
+  "kernel G H h = {x. elt\<^bsub>G\<^esub> x \<and> h\<langle>x\<rangle> = \<one>\<^bsub>H\<^esub>}"
+setup {* add_rewrite_rule @{thm kernel_def} *}
+
+theorem in_kernel [backward]: "elt\<^bsub>G\<^esub> x \<Longrightarrow> h\<langle>x\<rangle> = \<one>\<^bsub>H\<^esub> \<Longrightarrow> x \<in> kernel G H h" by auto2
+
+(* Earlier verified assumptions (such as \<forall>x\<in>H. inv x \<in> H) generate useless derivations. *)
+lemma kernel_is_subgroup [backward]:
+  "group G \<Longrightarrow> group H \<Longrightarrow> h \<in> hom G H \<Longrightarrow> is_subgroup (kernel G H h) G" by auto2
+
+lemma kernel_is_normal_subgroup:
+  "group G \<Longrightarrow> group H \<Longrightarrow> h \<in> hom G H \<Longrightarrow> is_normal_subgroup (kernel G H h) G" by auto2
+setup {* add_forward_prfstep_cond @{thm kernel_is_normal_subgroup} [with_term "kernel ?G ?H ?h"] *}
+
+theorem coset_non_empty [backward]: "H \<noteq> {} \<Longrightarrow> H #>\<^bsub>G\<^esub> a \<noteq> {}"
+  by (tactic {* auto2s_tac @{context}
+    (CHOOSE "h, h \<in> H" THEN OBTAIN "h \<otimes>\<^bsub>G\<^esub> a \<in> H #>\<^bsub>G\<^esub> a") *})
+
+definition set_hom ::
+  "('a, 'm) monoid_scheme \<Rightarrow> ('b, 'n) monoid_scheme \<Rightarrow> ('a \<Rightarrow> 'b) \<Rightarrow> ('a set \<Rightarrow> 'b)" where
+  "set_hom G H h S = the_elem (h ` S)"
+
+theorem set_hom_eval [rewrite]: "(set_hom G H h)\<langle>S\<rangle> = the_elem (h ` S)" by (simp add: set_hom_def)
+
+theorem set_hom_on_coset [rewrite]: fixes G (structure) shows
+  "group G \<Longrightarrow> group H \<Longrightarrow> elt a \<Longrightarrow> h \<in> hom G H \<Longrightarrow> (set_hom G H h)\<langle>(kernel G H h) #> a\<rangle> = h\<langle>a\<rangle>"
+  by (tactic {* auto2s_tac @{context}
+    (OBTAIN "\<forall>y\<in>(kernel G H h) #> a. h\<langle>y\<rangle> = h\<langle>a\<rangle>" WITH CHOOSE "x\<in>kernel G H h, y = x \<otimes> a") *})
+
+theorem set_hom_is_iso: fixes G (structure) shows
+  "group G \<Longrightarrow> group H \<Longrightarrow> h \<in> hom G H \<Longrightarrow> is_surj H h \<Longrightarrow> set_hom G H h \<in> (G Mod (kernel G H h)) \<cong> H"
+   by (tactic {* auto2s_tac @{context}
+     (CHOOSE "K, K = kernel G H h" THEN
+      CHOOSE "h', h' = set_hom G H h" THEN
+      OBTAIN "h' \<in> hom (G Mod K) H" THEN
+      OBTAIN "\<forall>S T. elt\<^bsub>G Mod K\<^esub> S \<longrightarrow> elt\<^bsub>G Mod K\<^esub> T \<longrightarrow> h'\<langle>S\<rangle> = h'\<langle>T\<rangle> \<longrightarrow> S = T" WITH
+       (CHOOSE "a, elt a \<and> S = K #> a" THEN
+        CHOOSE "b, elt b \<and> T = K #> b" THEN
+        OBTAIN "a \<otimes> inv b \<in> K") THEN
+      OBTAIN "\<forall>x. x \<in> image\<^bsub>G Mod K\<^esub> h' \<longleftrightarrow> x \<in> image h" WITH
+        CASE "x \<in> image h" WITH
+         (CHOOSE "y, elt y \<and> h\<langle>y\<rangle> = x" THEN
+          OBTAIN "x = (set_hom G H h)\<langle>(kernel G H h) #> y\<rangle>")) *})
+
+end
