Algebra_Ex/Group.thy
@@ -1,0 +1,300 @@
+(* Monoids and Groups, following HOL/Algebra/Group. *)
+
+theory Group
+imports Partial_Object
+begin
+
+subsection \<open>Monoids\<close>
+
+record 'a monoid = "'a partial_object" +
+  mult :: "'a \<Rightarrow> 'a \<Rightarrow> 'a" (infixl "\<otimes>\<index>" 70)
+  one :: 'a ("\<one>\<index>")
+
+definition monoid :: "('a, 'b) monoid_scheme \<Rightarrow> bool" where
+  "monoid G \<longleftrightarrow>
+    elt\<^bsub>G\<^esub> \<one>\<^bsub>G\<^esub> \<and>
+    (\<forall>x y. elt\<^bsub>G\<^esub> x \<longrightarrow> elt\<^bsub>G\<^esub> y \<longrightarrow> elt\<^bsub>G\<^esub> (x \<otimes>\<^bsub>G\<^esub> y)) \<and>
+    (\<forall>x y z. elt\<^bsub>G\<^esub> x \<longrightarrow> elt\<^bsub>G\<^esub> y \<longrightarrow> elt\<^bsub>G\<^esub> z \<longrightarrow> (x \<otimes>\<^bsub>G\<^esub> y) \<otimes>\<^bsub>G\<^esub> z = x \<otimes>\<^bsub>G\<^esub> (y \<otimes>\<^bsub>G\<^esub> z)) \<and>
+    (\<forall>x. elt\<^bsub>G\<^esub> x \<longrightarrow> \<one>\<^bsub>G\<^esub> \<otimes>\<^bsub>G\<^esub> x = x) \<and>
+    (\<forall>x. elt\<^bsub>G\<^esub> x \<longrightarrow> x \<otimes>\<^bsub>G\<^esub> \<one>\<^bsub>G\<^esub> = x)"
+setup {* add_property_const @{term "monoid"} *}
+
+lemma monoid_props: fixes G (structure) shows
+  "monoid G \<Longrightarrow> elt \<one>"
+  "monoid G \<Longrightarrow> elt x \<Longrightarrow> elt y \<Longrightarrow> elt (x \<otimes> y)"
+  "monoid G \<Longrightarrow> elt x \<Longrightarrow> elt y \<Longrightarrow> elt z \<Longrightarrow> (x \<otimes> y) \<otimes> z = x \<otimes> (y \<otimes> z)"
+  "monoid G \<Longrightarrow> elt x \<Longrightarrow> \<one> \<otimes> x = x"
+  "monoid G \<Longrightarrow> elt x \<Longrightarrow> x \<otimes> \<one> = x" by (simp add: Group.monoid_def struct_elt_def)+
+setup {* fold add_property_update @{thms monoid_props(1,2)} *}
+setup {* add_rewrite_rule_bidir_cond @{thm monoid_props(3)}
+  (with_conds ["?x \<noteq> \<one>\<^bsub>?G\<^esub>", "?y \<noteq> \<one>\<^bsub>?G\<^esub>", "?z \<noteq> \<one>\<^bsub>?G\<^esub>"]) *}
+setup {* fold add_rewrite_rule @{thms monoid_props(4,5)} *}
+
+setup {* add_backward_prfstep (equiv_backward_th @{thm monoid_def}) *}
+
+definition Units :: "_ \<Rightarrow> 'a set" -- \<open>The set of invertible elements\<close>
+  where "Units G = {x. elt\<^bsub>G\<^esub> x \<and> (\<exists>y. elt\<^bsub>G\<^esub> y \<and> y \<otimes>\<^bsub>G\<^esub> x = \<one>\<^bsub>G\<^esub> \<and> x \<otimes>\<^bsub>G\<^esub> y = \<one>\<^bsub>G\<^esub>)}"
+setup {* add_rewrite_rule @{thm Units_def} *}
+
+lemma Unit_closed [forward]: "x \<in> Units G \<Longrightarrow> elt\<^bsub>G\<^esub> x" by auto2
+
+lemma Unit_exists_inv [resolve]:
+  "x \<in> Units G \<Longrightarrow> \<exists>y. elt\<^bsub>G\<^esub> y \<and> y \<otimes>\<^bsub>G\<^esub> x = \<one>\<^bsub>G\<^esub> \<and> x \<otimes>\<^bsub>G\<^esub> y = \<one>\<^bsub>G\<^esub>" by auto2
+
+lemma Units_exists_invl [resolve]: "x \<in> Units G \<Longrightarrow> \<exists>y. elt\<^bsub>G\<^esub> y \<and> y \<otimes>\<^bsub>G\<^esub> x = \<one>\<^bsub>G\<^esub>" by auto2
+
+lemma Units_exists_invr [resolve]: "x \<in> Units G \<Longrightarrow> \<exists>y. elt\<^bsub>G\<^esub> y \<and> x \<otimes>\<^bsub>G\<^esub> y = \<one>\<^bsub>G\<^esub>" by auto2
+
+lemma Unit_intro [backward1, backward2]:
+  "elt\<^bsub>G\<^esub> x \<Longrightarrow> elt\<^bsub>G\<^esub> y \<Longrightarrow> y \<otimes>\<^bsub>G\<^esub> x = \<one>\<^bsub>G\<^esub> \<Longrightarrow> x \<otimes>\<^bsub>G\<^esub> y = \<one>\<^bsub>G\<^esub> \<Longrightarrow> x \<in> Units G" by auto2
+
+lemma Units_one_closed: fixes G (structure) shows
+  "monoid G \<Longrightarrow> \<one> \<in> Units G"
+  by (tactic {* auto2s_tac @{context} (OBTAIN "\<one> \<otimes> \<one> = \<one>") *})
+
+setup {* del_prfstep_thm @{thm Units_def} *}
+
+lemma Units_m_closed: fixes G (structure) shows
+  "monoid G \<Longrightarrow> x \<in> Units G \<Longrightarrow> y \<in> Units G \<Longrightarrow> x \<otimes> y \<in> Units G"
+  by (tactic {* auto2s_tac @{context}
+    (CHOOSE "x', elt x' \<and> x' \<otimes> x = \<one> \<and> x \<otimes> x' = \<one>" THEN
+     CHOOSE "y', elt y' \<and> y' \<otimes> y = \<one> \<and> y \<otimes> y' = \<one>" THEN
+     OBTAIN "(y' \<otimes> x') \<otimes> (x \<otimes> y) = \<one>" THEN
+     OBTAIN "(x \<otimes> y) \<otimes> (y' \<otimes> x') = \<one>") *})
+
+definition m_inv :: "('a, 'b) monoid_scheme \<Rightarrow> 'a \<Rightarrow> 'a" ("inv\<index> _" [81] 80)
+  where "inv\<^bsub>G\<^esub> x = (THE y. elt\<^bsub>G\<^esub> y \<and> y \<otimes>\<^bsub>G\<^esub> x = \<one>\<^bsub>G\<^esub> \<and> x \<otimes>\<^bsub>G\<^esub> y = \<one>\<^bsub>G\<^esub>)"
+setup {* add_rewrite_rule @{thm m_inv_def} *}
+
+lemma inv_unique [forward]: fixes G (structure) shows
+  "monoid G \<Longrightarrow> elt x \<Longrightarrow> elt y \<Longrightarrow> elt y' \<Longrightarrow> y \<otimes> x = \<one> \<Longrightarrow> x \<otimes> y' = \<one> \<Longrightarrow> y = y'"
+  by (tactic {* auto2s_tac @{context} (OBTAIN "y = y \<otimes> (x \<otimes> y')") *})
+
+theorem monoid_inv_prop: fixes G (structure) shows
+  "monoid G \<Longrightarrow> x \<in> Units G \<Longrightarrow> elt (inv x) \<and> inv x \<otimes> x = \<one> \<and> x \<otimes> inv x = \<one>"
+  by (tactic {* auto2s_tac @{context}
+    (OBTAIN "\<exists>!y. elt y \<and> y \<otimes> x = \<one> \<and> x \<otimes> y = \<one>") *})
+setup {* add_forward_prfstep_cond @{thm monoid_inv_prop} [with_term "inv\<^bsub>?G\<^esub> ?x"] *}
+setup {* del_prfstep_thm @{thm m_inv_def} *}
+
+theorem Units_inv_Units: "monoid G \<Longrightarrow> x \<in> Units G \<Longrightarrow> inv\<^bsub>G\<^esub> x \<in> Units G" by auto2
+setup {* add_forward_prfstep_cond @{thm Units_inv_Units} [with_term "inv\<^bsub>?G\<^esub> ?x"] *}
+
+lemma Units_l_cancel [forward]: fixes G (structure) shows
+  "monoid G \<Longrightarrow> elt y \<Longrightarrow> elt z \<Longrightarrow> x \<otimes> y = x \<otimes> z \<Longrightarrow> x \<in> Units G \<Longrightarrow> y = z"
+  by (tactic {* auto2s_tac @{context} (OBTAIN "(inv x \<otimes> x) \<otimes> y = (inv x \<otimes> x) \<otimes> z") *})
+
+lemma Units_r_cancel [forward]: fixes G (structure) shows
+  "monoid G \<Longrightarrow> elt y \<Longrightarrow> elt z \<Longrightarrow> y \<otimes> x = z \<otimes> x \<Longrightarrow> x \<in> Units G \<Longrightarrow> y = z"
+  by (tactic {* auto2s_tac @{context} (OBTAIN "y \<otimes> (x \<otimes> inv x) = z \<otimes> (x \<otimes> inv x)") *})
+
+lemma Units_inv_inv [rewrite]: fixes G (structure) shows
+  "monoid G \<Longrightarrow> x \<in> Units G \<Longrightarrow> inv (inv x) = x" by auto2
+
+lemma inv_inj_on_Units: "monoid G \<Longrightarrow> inj_on (m_inv G) (Units G)" by auto2
+
+lemma Units_inv_comm [backward2]: fixes G (structure) shows
+  "monoid G \<Longrightarrow> elt y \<Longrightarrow> x \<otimes> y = \<one> \<Longrightarrow> x \<in> Units G \<Longrightarrow> y \<otimes> x = \<one>"
+  by (tactic {* auto2s_tac @{context} (OBTAIN "x \<otimes> y \<otimes> x = x \<otimes> \<one>") *})
+
+lemma monoid_set_not_empty: fixes G (structure) shows
+  "monoid G \<Longrightarrow> \<exists>x. elt x"
+  by (tactic {* auto2s_tac @{context} (OBTAIN "elt \<one>") *})
+
+definition order :: "('a, 'b) monoid_scheme \<Rightarrow> nat" where
+  "order S = card (carrier S)"
+setup {* add_rewrite_rule @{thm order_def} *}
+
+subsection \<open>Groups\<close>
+
+definition group :: "('a, 'b) monoid_scheme \<Rightarrow> bool" where
+  "group G \<longleftrightarrow> monoid G \<and> (\<forall>x. elt\<^bsub>G\<^esub> x \<longrightarrow> x \<in> Units G)"
+setup {* add_property_const @{term "group"} *}
+
+setup {* add_backward_prfstep (equiv_backward_th @{thm group_def}) *}
+theorem groupI [backward]: fixes G (structure) shows
+  "monoid G \<Longrightarrow> \<forall>x. elt x \<longrightarrow> (\<exists>y. elt y \<and> y \<otimes> x = \<one>) \<Longrightarrow> group G"
+  by (tactic {* auto2s_tac @{context}
+    (* First show the left-cancellation property *)
+    (OBTAIN "\<forall>x y z. elt x \<longrightarrow> elt y \<longrightarrow> elt z \<longrightarrow> x \<otimes> y = x \<otimes> z \<longrightarrow> y = z" WITH
+      (CHOOSE "x', elt x' \<and> x' \<otimes> x = \<one>" THEN
+       OBTAIN "x' \<otimes> x \<otimes> y = x' \<otimes> x \<otimes> z") THEN
+    (* Key idea is that y \<otimes> x = \<one> implies x \<otimes> y = \<one> *)
+    (OBTAIN "\<forall>x. elt x \<longrightarrow> x \<in> Units G" WITH
+      (CHOOSE "y, elt y \<and> y \<otimes> x = \<one>" THEN
+       OBTAIN "y \<otimes> x \<otimes> y = y \<otimes> \<one>"))) *})
+setup {* del_prfstep_thm @{thm group_def} #>
+  add_forward_prfstep_cond (equiv_forward_th @{thm group_def}) [with_term "?G"] *}
+
+theorem group_to_monoid: "group G \<Longrightarrow> monoid G" by auto2
+setup {* add_property_update @{thm group_to_monoid} *}
+theorem group_elt_is_unit: "group G \<Longrightarrow> elt\<^bsub>G\<^esub> x \<Longrightarrow> x \<in> Units G" by auto2
+setup {* add_forward_prfstep_cond @{thm group_elt_is_unit} [with_term "?x", with_term "?G"] *}
+
+(* Since every element is a unit, can streamline proofs here *)
+theorem group_inv_prop: fixes G (structure) shows
+  "group G \<Longrightarrow> elt x \<Longrightarrow> elt (inv x) \<and> inv x \<otimes> x = \<one> \<and> x \<otimes> inv x = \<one>" by auto2
+setup {* add_property_update (conj_left_th @{thm group_inv_prop}) *}
+setup {* add_rewrite_rule (conj_left_th (conj_right_th @{thm group_inv_prop})) *}
+setup {* add_rewrite_rule (conj_right_th (conj_right_th @{thm group_inv_prop})) *}
+
+theorem group_l_cancel [forward]: fixes G (structure) shows
+  "group G \<Longrightarrow> elt x \<Longrightarrow> elt y \<Longrightarrow> elt z \<Longrightarrow> x \<otimes> y = x \<otimes> z \<Longrightarrow> y = z" by auto2
+
+theorem group_r_cancel [forward]: fixes G (structure) shows
+  "group G \<Longrightarrow> elt x \<Longrightarrow> elt y \<Longrightarrow> elt z \<Longrightarrow> y \<otimes> x = z \<otimes> x \<Longrightarrow> y = z" by auto2
+
+lemma group_inv_inv [rewrite]: fixes G (structure) shows
+  "group G \<Longrightarrow> elt x \<Longrightarrow> inv (inv x) = x" by auto2
+
+setup {* fold del_prfstep_thm [@{thm group_def}, @{thm group_elt_is_unit}] *}
+
+theorem inv_equality [backward]: fixes G (structure) shows
+  "group G \<Longrightarrow> elt x \<Longrightarrow> elt y \<Longrightarrow> y \<otimes> x = \<one> \<Longrightarrow> inv x = y"
+  by (tactic {* auto2s_tac @{context} (OBTAIN "inv x \<otimes> x = \<one>") *})
+
+lemma inv_mult_group: fixes G (structure) shows
+  "group G \<Longrightarrow> elt x \<Longrightarrow> elt y \<Longrightarrow> inv (x \<otimes> y) = inv y \<otimes> inv x" by auto2
+setup {* add_rewrite_rule_cond @{thm inv_mult_group} (with_conds ["?x \<noteq> \<one>\<^bsub>?G\<^esub>", "?y \<noteq> \<one>\<^bsub>?G\<^esub>"]) *}
+
+theorem move_inv_r: fixes G (structure) shows
+  "group G \<Longrightarrow> elt a \<Longrightarrow> elt b \<Longrightarrow> elt c \<Longrightarrow> a \<otimes> inv b = c \<longleftrightarrow> a = c \<otimes> b" by auto2
+setup {* add_rewrite_rule_cond @{thm move_inv_r} [with_cond "?b \<noteq> \<one>\<^bsub>?G\<^esub>"] *}
+
+theorem move_inv_l: fixes G (structure) shows
+  "group G \<Longrightarrow> elt a \<Longrightarrow> elt b \<Longrightarrow> elt c \<Longrightarrow> inv a \<otimes> b = c \<longleftrightarrow> b = a \<otimes> c" by auto2
+setup {* add_rewrite_rule_cond @{thm move_inv_l} [with_cond "?a \<noteq> \<one>\<^bsub>?G\<^esub>"] *}
+
+subsection \<open>Subgroups\<close>
+
+definition is_subgroup :: "'a set \<Rightarrow> ('a, 'b) monoid_scheme \<Rightarrow> bool" where
+  "is_subgroup H G \<longleftrightarrow>
+    group G \<and>
+    subset\<^bsub>G\<^esub> H \<and>
+    (\<forall>x y. x \<in> H \<longrightarrow> y \<in> H \<longrightarrow> x \<otimes>\<^bsub>G\<^esub> y \<in> H) \<and>
+    (\<one>\<^bsub>G\<^esub> \<in> H) \<and>
+    (\<forall>x\<in>H. inv\<^bsub>G\<^esub> x \<in> H)"
+
+definition subgroup :: "'a set \<Rightarrow> ('a, 'b) monoid_scheme \<Rightarrow> ('a, 'b) monoid_scheme" where
+  "subgroup H G = G \<lparr>carrier := H\<rparr>"
+
+lemma subgroup_sel:
+  "elt\<^bsub>subgroup H G\<^esub> x \<longleftrightarrow> x \<in> H"
+  "x \<otimes>\<^bsub>subgroup H G\<^esub> y = x \<otimes>\<^bsub>G\<^esub> y"
+  "\<one>\<^bsub>subgroup H G\<^esub> = \<one>\<^bsub>G\<^esub>" by (simp add: subgroup_def struct_elt_def)+
+setup {* add_forward_prfstep_cond (equiv_forward_th @{thm subgroup_sel(1)}) [with_term "?x", with_term "is_subgroup ?H ?G"] *}
+setup {* add_forward_prfstep_cond (equiv_backward_th @{thm subgroup_sel(1)}) [with_term "is_subgroup ?H ?G"] *}
+setup {* fold add_rewrite_rule @{thms subgroup_sel(2-3)} *}
+
+setup {* add_rewrite_rule @{thm is_subgroup_def} *}
+lemma is_subgroupI [backward]: fixes G (structure) shows
+  "group G \<Longrightarrow> subset\<^bsub>G\<^esub> H \<Longrightarrow> \<forall>x y. x \<in> H \<longrightarrow> y \<in> H \<longrightarrow> x \<otimes> y \<in> H \<Longrightarrow>
+   \<one> \<in> H \<Longrightarrow> \<forall>x\<in>H. inv x \<in> H \<Longrightarrow> is_subgroup H G" by auto2
+setup {* del_prfstep_thm @{thm is_subgroup_def} *}
+
+lemma is_subgroupD:
+  "is_subgroup H G \<Longrightarrow> group G"
+  "is_subgroup H G \<Longrightarrow> subset\<^bsub>G\<^esub> H"
+  "elt\<^bsub>subgroup H G\<^esub>x \<Longrightarrow> elt\<^bsub>subgroup H G\<^esub>y \<Longrightarrow> is_subgroup H G \<Longrightarrow> x \<otimes>\<^bsub>G\<^esub> y \<in> H"
+  "is_subgroup H G \<Longrightarrow> \<one>\<^bsub>G\<^esub> \<in> H"
+  "elt\<^bsub>subgroup H G\<^esub>x \<Longrightarrow> is_subgroup H G \<Longrightarrow> inv\<^bsub>G\<^esub> x \<in> H" by (simp add: subgroup_def is_subgroup_def struct_elt_def)+
+setup {* fold add_forward_prfstep @{thms is_subgroupD(1-2)} *}
+setup {* add_forward_prfstep_cond @{thm is_subgroupD(3)} [with_term "?x \<otimes>\<^bsub>?G\<^esub> ?y"] *}
+setup {* add_forward_prfstep_cond @{thm is_subgroupD(4)} [with_term "\<one>\<^bsub>?G\<^esub>"] *}
+setup {* add_forward_prfstep_cond @{thm is_subgroupD(5)} [with_term "inv\<^bsub>?G\<^esub> ?x"] *}
+
+lemma subgroup_is_group: "is_subgroup H G \<Longrightarrow> group (subgroup H G)"
+  by (tactic {* auto2s_tac @{context}
+    (CHOOSE "\<H>, \<H> = subgroup H G" THEN
+     OBTAIN "monoid \<H>" THEN
+     OBTAIN "\<forall>x. elt\<^bsub>\<H>\<^esub> x \<longrightarrow> (\<exists>y. elt\<^bsub>\<H>\<^esub> y \<and> y \<otimes>\<^bsub>\<H>\<^esub> x = \<one>\<^bsub>\<H>\<^esub>)" WITH
+      (OBTAIN "inv\<^bsub>G\<^esub> x \<otimes>\<^bsub>\<H>\<^esub> x = \<one>\<^bsub>\<H>\<^esub>")) *})
+
+theorem subgroup_non_empty [resolve]: "is_subgroup H G \<Longrightarrow> H \<noteq> {}"
+  by (tactic {* auto2s_tac @{context} (OBTAIN "\<one>\<^bsub>G\<^esub> \<in> H") *})
+
+subsection \<open>Direct Products\<close>
+
+definition DirProd :: "_ \<Rightarrow> _ \<Rightarrow> ('a \<times> 'b) monoid" (infixr "\<times>\<times>" 80) where
+  "G \<times>\<times> H =
+    \<lparr>carrier = carrier G \<times> carrier H,
+     mult = (\<lambda>(g, h) (g', h'). (g \<otimes>\<^bsub>G\<^esub> g', h \<otimes>\<^bsub>H\<^esub> h')),
+     one = (\<one>\<^bsub>G\<^esub>, \<one>\<^bsub>H\<^esub>)\<rparr>"
+
+lemma Dir_Prod_sel:
+  "elt\<^bsub>G \<times>\<times> H\<^esub> (g, h) \<longleftrightarrow> elt\<^bsub>G\<^esub> g \<and> elt\<^bsub>H\<^esub> h"
+  "\<one>\<^bsub>G \<times>\<times> H\<^esub> = (\<one>\<^bsub>G\<^esub>, \<one>\<^bsub>H\<^esub>)"
+  "(g, h) \<otimes>\<^bsub>(G \<times>\<times> H)\<^esub> (g', h') = (g \<otimes>\<^bsub>G\<^esub> g', h \<otimes>\<^bsub>H\<^esub> h')" by (simp add: DirProd_def struct_elt_def)+
+setup {* add_backward_prfstep (equiv_backward_th @{thm Dir_Prod_sel(1)}) *}
+setup {* fold add_rewrite_rule @{thms Dir_Prod_sel(2,3)} *}
+
+theorem elt_prod: "elt\<^bsub>G\<^esub> x \<Longrightarrow> elt\<^bsub>H\<^esub> y \<Longrightarrow> elt\<^bsub>G \<times>\<times> H\<^esub> (x, y)"
+  by (simp add: Dir_Prod_sel(1))
+setup {* add_forward_prfstep_cond @{thm elt_prod} [with_term "(?x, ?y)", with_term "?G \<times>\<times> ?H"] *}
+theorem Prod_eq [backward1]: "x = x' \<Longrightarrow> y = y' \<Longrightarrow> (x, y) = (x', y')" by auto
+theorem mem_DirProd: "elt\<^bsub>G \<times>\<times> H\<^esub> x \<Longrightarrow> x = (fst x, snd x) \<and> elt\<^bsub>G\<^esub> (fst x) \<and> elt\<^bsub>H\<^esub> (snd x)"
+  by (metis Dir_Prod_sel(1) prod.collapse)
+setup {* add_forward_prfstep_cond @{thm mem_DirProd}
+  (with_term "?x" :: with_term "?G \<times>\<times> ?H" :: with_conds ["?x \<noteq> (?x1, ?x2)", "?x \<noteq> \<one>\<^bsub>?G \<times>\<times> ?H\<^esub>"]) *}
+
+(* Takes a long time here *)
+lemma DirProd_monoid: "monoid G \<Longrightarrow> monoid H \<Longrightarrow> monoid (G \<times>\<times> H)" by auto2
+setup {* add_forward_prfstep_cond @{thm DirProd_monoid} [with_term "?G \<times>\<times> ?H"] *}
+
+lemma DirProd_group: "group G \<Longrightarrow> group H \<Longrightarrow> group (G \<times>\<times> H)"
+  by (tactic {* auto2s_tac @{context}
+    (CHOOSE "A, A = G \<times>\<times> H" THEN
+     OBTAIN "monoid A" THEN
+     OBTAIN "\<forall>x. elt\<^bsub>A\<^esub> x \<longrightarrow> (\<exists>y. elt\<^bsub>A\<^esub> y \<and> y \<otimes>\<^bsub>A\<^esub> x = \<one>\<^bsub>A\<^esub>)" WITH
+       OBTAIN "(inv\<^bsub>G\<^esub> (fst x), inv\<^bsub>H\<^esub> (snd x)) \<otimes>\<^bsub>A\<^esub> x = \<one>\<^bsub>A\<^esub>") *})
+setup {* add_forward_prfstep_cond @{thm DirProd_group} [with_term "?G \<times>\<times> ?H"] *}
+
+lemma inv_DirProd [rewrite]: "group G \<Longrightarrow> group H \<Longrightarrow> elt\<^bsub>G\<^esub> g \<Longrightarrow> elt\<^bsub>H\<^esub> h \<Longrightarrow>
+  inv\<^bsub>G \<times>\<times> H\<^esub> (g, h) = (inv\<^bsub>G\<^esub> g, inv\<^bsub>H\<^esub> h)" by auto2
+
+subsection \<open>Homomorphisms and Isomorphisms\<close>
+
+definition hom :: "_ \<Rightarrow> _ \<Rightarrow> ('a \<Rightarrow> 'b) set" where
+  "hom G H =
+    {h. h \<in> carrier G \<rightarrow> carrier H \<and>
+      (\<forall>x y. elt\<^bsub>G\<^esub> x \<longrightarrow> elt\<^bsub>G\<^esub> y \<longrightarrow> h \<langle>x \<otimes>\<^bsub>G\<^esub> y\<rangle> = h\<langle>x\<rangle> \<otimes>\<^bsub>H\<^esub> h\<langle>y\<rangle>)}"
+
+theorem is_homD1: "elt\<^bsub>G\<^esub> x \<Longrightarrow> h \<in> hom G H \<Longrightarrow> elt\<^bsub>H\<^esub> h\<langle>x\<rangle>"
+  by (metis (no_types, lifting) Pi_mem feval_def hom_def struct_elt_def mem_Collect_eq)
+setup {* add_forward_prfstep_cond @{thm is_homD1} [with_term "?h\<langle>?x\<rangle>"] *}
+
+theorem is_homD2 [rewrite]:
+  "elt\<^bsub>G\<^esub> x \<Longrightarrow> elt\<^bsub>G\<^esub> y \<Longrightarrow> h \<in> hom G H \<Longrightarrow> h \<langle>x \<otimes>\<^bsub>G\<^esub> y\<rangle> = h\<langle>x\<rangle> \<otimes>\<^bsub>H\<^esub> h\<langle>y\<rangle>"
+  by (simp add: hom_def struct_elt_def)
+
+theorem is_homI [backward]:
+  "\<forall>x. elt\<^bsub>G\<^esub> x \<longrightarrow> elt\<^bsub>H\<^esub> h\<langle>x\<rangle> \<Longrightarrow> \<forall>x y. elt\<^bsub>G\<^esub> x \<longrightarrow> elt\<^bsub>G\<^esub> y \<longrightarrow> h \<langle>x \<otimes>\<^bsub>G\<^esub> y\<rangle> = h\<langle>x\<rangle> \<otimes>\<^bsub>H\<^esub> h\<langle>y\<rangle> \<Longrightarrow>
+   h \<in> hom G H" by (simp add: hom_def struct_elt_def)
+
+lemma hom_compose [backward1]:
+  "group G \<Longrightarrow> h \<in> hom G H \<Longrightarrow> i \<in> hom H I \<Longrightarrow> i \<circ>\<^bsub>G\<^esub> h \<in> hom G I" by auto2
+
+lemma hom_one_closed [rewrite]: fixes G (structure) shows
+  "group G \<Longrightarrow> group H \<Longrightarrow> h \<in> hom G H \<Longrightarrow> h\<langle>\<one>\<rangle> = \<one>\<^bsub>H\<^esub>"
+  by (tactic {* auto2s_tac @{context} (OBTAIN "h\<langle>\<one> \<otimes> \<one>\<rangle> = h\<langle>\<one>\<rangle> \<otimes>\<^bsub>H\<^esub> \<one>\<^bsub>H\<^esub>") *})
+
+lemma hom_inv_closed [rewrite]: fixes G (structure) shows
+  "group G \<Longrightarrow> group H \<Longrightarrow> elt x \<Longrightarrow> h \<in> hom G H \<Longrightarrow> h\<langle>inv x\<rangle> = inv\<^bsub>H\<^esub> h\<langle>x\<rangle>"
+  by (tactic {* auto2s_tac @{context} (OBTAIN "h\<langle>inv x \<otimes> x\<rangle> = \<one>\<^bsub>H\<^esub>") *})
+
+definition iso :: "_ \<Rightarrow> _ \<Rightarrow> ('a \<Rightarrow> 'b) set" (infixr "\<cong>" 60) where
+  "G \<cong> H = {h. h \<in> hom G H \<and> struct_is_bij G H h}"
+setup {* add_rewrite_rule @{thm iso_def} *}
+
+lemma iso_refl: "(\<lambda>x. x) \<in> G \<cong> G" by auto2
+
+lemma iso_trans: "group G \<Longrightarrow> h \<in> G \<cong> H \<Longrightarrow> i \<in> H \<cong> I \<Longrightarrow> (i \<circ>\<^bsub>G\<^esub> h) \<in> G \<cong> I" by auto2
+
+lemma iso_sym: "group G \<Longrightarrow> group H \<Longrightarrow> h \<in> G \<cong> H \<Longrightarrow> inv_fun\<^bsub>G\<^esub> h \<in> H \<cong> G"
+  by (tactic {* auto2s_tac @{context}
+    (CHOOSE "h', h' = inv_fun\<^bsub>G\<^esub> h" THEN
+     OBTAIN "\<forall>x y. elt\<^bsub>H\<^esub> x \<longrightarrow> elt\<^bsub>H\<^esub> y \<longrightarrow> h' \<langle>x \<otimes>\<^bsub>H\<^esub> y\<rangle> = (h'\<langle>x\<rangle>) \<otimes>\<^bsub>G\<^esub> (h'\<langle>y\<rangle>)" WITH
+      (OBTAIN "h \<langle>h' \<langle>x \<otimes>\<^bsub>H\<^esub> y\<rangle>\<rangle> = x \<otimes>\<^bsub>H\<^esub> y" THEN
+       OBTAIN "h \<langle>h'\<langle>x\<rangle> \<otimes>\<^bsub>G\<^esub> h'\<langle>y\<rangle>\<rangle> = x \<otimes>\<^bsub>H\<^esub> y")) *})
+
+end
