Algebra_Ex/Partial_Object.thy
@@ -1,0 +1,109 @@
+theory Partial_Object
+imports Prelim_Thms Feval
+begin
+
+(* Use only in this theory *)
+setup {* add_rewrite_rule @{thm inj_on_def} *}
+setup {* add_rewrite_rule @{thm feval_def} *}
+setup {* add_backward_prfstep @{thm set_ext} *}
+
+subsection \<open>Partial objects\<close>
+
+record 'a partial_object =
+  carrier :: "'a set"
+
+definition struct_elt :: "_ \<Rightarrow> 'a \<Rightarrow> bool"  ("elt\<index> _" [81] 80) where
+  "elt\<^bsub>G\<^esub> x \<longleftrightarrow> x \<in> carrier G"
+setup {* add_rewrite_rule @{thm struct_elt_def} *}
+setup {* add_forward_prfstep (equiv_backward_th @{thm struct_elt_def}) *}
+setup {* add_backward_prfstep (equiv_forward_th @{thm struct_elt_def}) *}
+
+definition struct_subset :: "_ \<Rightarrow> 'a set \<Rightarrow> bool"  ("subset\<index> _" [81] 80) where
+  "subset\<^bsub>G\<^esub> H \<longleftrightarrow> (\<forall>x\<in>H. elt\<^bsub>G\<^esub> x)"
+setup {* add_backward_prfstep (equiv_backward_th @{thm struct_subset_def}) *}
+
+theorem struct_subsetE [forward]: "subset\<^bsub>G\<^esub> H \<Longrightarrow> x \<in> H \<Longrightarrow> elt\<^bsub>G\<^esub> x"
+  by (simp add: struct_subset_def)
+
+definition struct_compose :: "_ \<Rightarrow> ('b \<Rightarrow> 'c) \<Rightarrow> ('a \<Rightarrow> 'b) \<Rightarrow> 'a \<Rightarrow> 'c" (infixr "\<circ>\<index>" 55) where
+  "i \<circ>\<^bsub>G\<^esub> h = compose (carrier G) i h"
+setup {* add_rewrite_rule @{thm struct_compose_def} *}
+
+theorem struct_compose_eq [rewrite]: "elt\<^bsub>G\<^esub> x \<Longrightarrow> (g \<circ>\<^bsub>G\<^esub> f)\<langle>x\<rangle> = g\<langle>f\<langle>x\<rangle>\<rangle>" by auto2
+
+definition struct_is_inj :: "_ \<Rightarrow> ('a \<Rightarrow> 'b) \<Rightarrow> bool"  ("is'_inj\<index> _" [81] 80) where
+  "is_inj\<^bsub>G\<^esub> h \<longleftrightarrow> inj_on h (carrier G)"
+setup {* add_rewrite_rule_bidir @{thm struct_is_inj_def} *}
+
+definition struct_is_surj :: "_ \<Rightarrow> _ \<Rightarrow> ('a \<Rightarrow> 'b) \<Rightarrow> bool" ("is'_surj\<index> _ _" [81, 80] 80) where
+  "is_surj\<^bsub>G\<^esub> H h \<longleftrightarrow> h ` carrier G = carrier H"
+setup {* add_rewrite_rule_bidir @{thm struct_is_surj_def} *}
+
+theorem struct_is_inj_def': "is_inj\<^bsub>G\<^esub> h \<longleftrightarrow> (\<forall>x y. elt\<^bsub>G\<^esub> x \<longrightarrow> elt\<^bsub>G\<^esub>y \<longrightarrow> h\<langle>x\<rangle> = h\<langle>y\<rangle> \<longrightarrow> x = y)" by auto2
+setup {* add_forward_prfstep (equiv_backward_th @{thm struct_is_inj_def'}) *}
+
+definition struct_image :: "_ \<Rightarrow> ('a \<Rightarrow> 'b) \<Rightarrow> 'b set"  ("image\<index> _" [81] 80) where
+  "image\<^bsub>G\<^esub> h = {y. \<exists>x. elt\<^bsub>G\<^esub> x \<and> h\<langle>x\<rangle> = y}"
+setup {* add_rewrite_rule @{thm struct_image_def} *}
+
+theorem struct_is_surj_image_def: fixes G (structure) shows
+  "is_surj H h \<longleftrightarrow> (\<forall>x. elt x \<longrightarrow> elt\<^bsub>H\<^esub> h\<langle>x\<rangle>) \<and> image h = carrier H" by auto2
+setup {* add_backward_prfstep (equiv_backward_th @{thm struct_is_surj_image_def}) *}
+setup {* add_forward_prfstep (conj_right_th (equiv_forward_th @{thm struct_is_surj_image_def})) *}
+
+theorem mem_imageI: "h\<langle>x\<rangle> = y \<Longrightarrow> elt\<^bsub>G\<^esub> x \<Longrightarrow> y \<in> image\<^bsub>G\<^esub> h" by auto2
+setup {* add_forward_prfstep_cond @{thm mem_imageI} [with_term "image\<^bsub>?G\<^esub> ?h"] *}
+
+theorem mem_imageD [forward]: "y \<in> image\<^bsub>G\<^esub> h \<Longrightarrow> \<exists>x. elt\<^bsub>G\<^esub> x \<and> h\<langle>x\<rangle> = y" by auto2
+
+definition struct_is_bij :: "_ \<Rightarrow> _ \<Rightarrow> ('a \<Rightarrow> 'b) \<Rightarrow> bool" where
+  "struct_is_bij G H h \<longleftrightarrow> is_inj\<^bsub>G\<^esub> h \<and> is_surj\<^bsub>G\<^esub> H h"
+setup {* add_forward_prfstep (equiv_forward_th @{thm struct_is_bij_def}) *}
+setup {* add_rewrite_rule @{thm struct_is_bij_def} *}
+
+theorem struct_is_bij_def' [rewrite_bidir]:
+  "struct_is_bij G H h \<longleftrightarrow> bij_betw h (carrier G) (carrier H)" by auto2
+
+theorem struct_is_bijI [backward2]:
+  "is_inj\<^bsub>G\<^esub> h \<Longrightarrow> is_surj\<^bsub>G\<^esub> H h \<Longrightarrow> struct_is_bij G H h" by auto2
+
+theorem struct_is_bij_identity [resolve]: "struct_is_bij G G (\<lambda>x. x)" by auto2
+
+theorem struct_is_bij_transitive [backward2]:
+  "struct_is_bij G H f \<Longrightarrow> struct_is_bij H I g \<Longrightarrow> struct_is_bij G I (g \<circ>\<^bsub>G\<^esub> f)" by auto2
+
+definition struct_inv_into :: "_ \<Rightarrow> ('a \<Rightarrow> 'b) \<Rightarrow> ('b \<Rightarrow> 'a)" ("inv'_fun\<index> _" [81] 80) where
+  "inv_fun\<^bsub>G\<^esub> f = inv_into (carrier G) f"
+setup {* add_rewrite_rule @{thm struct_inv_into_def} *}
+
+theorem struct_inv_into_eval:
+  "f\<langle>x\<rangle> = y \<Longrightarrow> is_inj\<^bsub>G\<^esub> f \<Longrightarrow> elt\<^bsub>G\<^esub> x \<Longrightarrow> (inv_fun\<^bsub>G\<^esub> f)\<langle>y\<rangle> = x" by auto2
+setup {* add_forward_prfstep_cond @{thm struct_inv_into_eval} [with_term "(inv_fun\<^bsub>?G\<^esub> ?f)\<langle>?y\<rangle>"] *}
+
+theorem struct_inv_into_mem:
+  "is_surj\<^bsub>G\<^esub> H f \<Longrightarrow> elt\<^bsub>H\<^esub> x \<Longrightarrow> elt\<^bsub>G\<^esub> (inv_fun\<^bsub>G\<^esub> f)\<langle>x\<rangle>" by auto2
+setup {* add_forward_prfstep_cond @{thm struct_inv_into_mem} [with_term "(inv_fun\<^bsub>?G\<^esub> ?f)\<langle>?x\<rangle>"] *}
+
+theorem struct_bij_betw_inv_into_right' [rewrite]:
+  "struct_is_bij G H f \<Longrightarrow> elt\<^bsub>H\<^esub> y \<Longrightarrow> f \<langle>(inv_fun\<^bsub>G\<^esub> f) \<langle>y\<rangle>\<rangle> = y" by auto2
+
+theorem struct_bij_inv_fun [backward]:
+  "struct_is_bij G H f \<Longrightarrow> struct_is_bij H G (inv_fun\<^bsub>G\<^esub> f)" by auto2
+
+(* Remove proof steps added for this theory. *)
+setup {* fold del_prfstep ["Fun.inj_on_def", "Feval.feval_def", "Logic_Thms.set_ext@back"] *}
+
+(* Remove part of definition of struct_elt and strict_is_bij. *)
+setup {* fold del_prfstep ["Partial_Object.struct_elt_def", "Partial_Object.struct_is_bij_def"] *}
+
+(* Remove all uses of definition of several other theorems. *)
+setup {* fold del_prfstep_thm [
+  @{thm struct_compose_def},
+  @{thm struct_is_inj_def}, @{thm struct_is_surj_def},
+  @{thm struct_is_bij_def'}, @{thm struct_inv_into_def}]
+*}
+
+(* Declare elt as property constant. *)
+setup {* add_property_const @{term "struct_elt"} *}
+
+end
