Analysis/Rat_Thms.thy
@@ -7,22 +7,24 @@ begin
 subsection {* Basic properties of absolute values *}
 
 setup {* add_rewrite_rule @{thm abs_zero} *}
-setup {* add_resolve_prfstep @{thm abs_ge_zero} *}
+setup {* add_resolve_prfstep @{thm abs_not_less_zero} *}
 setup {* add_rewrite_rule @{thm abs_minus_cancel} *}
+setup {* add_rewrite_rule @{thm abs_minus_commute} *}
 setup {* add_rewrite_rule @{thm abs_of_pos} *}
 setup {* add_rewrite_rule @{thm abs_of_neg} *}
 setup {* add_rewrite_rule @{thm zero_less_abs_iff} *}
-setup {* add_rewrite_rule_cond @{thm abs_mult}
-  [with_filt (canonical_split_filter @{const_name times} "a" "b")] *}
-setup {* add_rewrite_rule_cond @{thm abs_inverse}
-  [with_filt (ac_atomic_filter @{const_name times} "a")] *}
+setup {* add_rewrite_rule @{thm abs_mult} *}
+setup {* add_rewrite_rule @{thm abs_inverse} *}
 setup {* add_rewrite_rule @{thm abs_numeral} *}
 lemma abs_ge_cases [forward]: fixes x :: "'a::linordered_idom"
   shows "\<bar>x\<bar> \<ge> r \<Longrightarrow> x > -r \<Longrightarrow> x \<ge> r" "\<bar>x\<bar> \<ge> r \<Longrightarrow> x < r \<Longrightarrow> x \<le> -r" by arith+
 lemma abs_gt_cases [forward]: fixes x :: "'a::linordered_idom"
   shows "\<bar>x\<bar> > r \<Longrightarrow> x \<ge> -r \<Longrightarrow> x > r" "\<bar>x\<bar> > r \<Longrightarrow> x \<le> r \<Longrightarrow> x < -r" by arith+
-setup {* add_forward_prfstep (equiv_forward_th @{thm abs_le_iff}) *}
-setup {* add_forward_prfstep (equiv_forward_th @{thm abs_less_iff}) *}
+theorem abs_le_on_diff: "\<bar>(a::('a::linordered_idom)) - b\<bar> \<le> r \<Longrightarrow> a \<le> b + r \<and> b \<le> a + r" by auto
+setup {* add_forward_prfstep_cond @{thm abs_le_on_diff} [with_filt (order_filter "a" "b"), with_cond "?a \<noteq> ?b", with_cond "?r \<noteq> 0"] *}
+theorem abs_less_on_diff: "\<bar>(a::('a::linordered_idom)) - b\<bar> < r \<Longrightarrow> a < b + r \<and> b < a + r" by auto
+setup {* add_forward_prfstep_cond @{thm abs_less_on_diff} [with_filt (order_filter "a" "b"), with_cond "?a \<noteq> ?b", with_cond "?r \<noteq> 0"] *}
+theorem abs_le_zero [forward]: "\<bar>(a::('a::linordered_idom)) - b\<bar> \<le> 0 \<Longrightarrow> a = b" by simp
 theorem abs_diff_nonneg [rewrite]: "(a::('a::linordered_idom)) \<ge> b \<Longrightarrow> \<bar>a - b\<bar> = a - b" by simp
 
 (* Shifting negation to the other side of inequality. *)
@@ -37,13 +39,16 @@ ML_file "rat_arith_test.ML"
 subsection {* Equalities on rationals *}
 
 theorem divide_cancel_gt0 [rewrite]:
-  "(a::('a::linordered_field)) > 0 \<Longrightarrow> bu * a * inverse a = bu" by simp
+  "(a::('a::linordered_field)) > 0 \<Longrightarrow> a * inverse a * bu = bu" by simp
 
-lemma diff_inverse: "(a::('a::field)) \<noteq> 0 \<Longrightarrow> b \<noteq> 0 \<Longrightarrow> inverse a - inverse b = (b-a)/(a*b)"
+lemma diff_inverse: "(a::('a::field)) \<noteq> 0 \<Longrightarrow> b \<noteq> 0 \<Longrightarrow> 1 / a - 1 / b = (b-a)/(a*b)"
   by (simp add: diff_divide_distrib inverse_eq_divide)
 lemma diff_inverse_bound [backward2]:
-  "(a::('a::linordered_field)) \<noteq> 0 \<Longrightarrow> b \<noteq> 0 \<Longrightarrow> \<bar>inverse a - inverse b\<bar> = \<bar>a-b\<bar>/\<bar>a*b\<bar>"
+  "(a::('a::linordered_field)) \<noteq> 0 \<Longrightarrow> b \<noteq> 0 \<Longrightarrow> \<bar>1 / a - 1 / b\<bar> = \<bar>a-b\<bar>/\<bar>a*b\<bar>"
   by (simp add: abs_minus_commute diff_inverse)
+
+theorem divide_by_numc [rewrite]: "(a::'a::linordered_field) / NUMC = a * inverse NUMC" by algebra
+setup {* add_rewrite_rule @{thm diff_minus_eq_add} *}
 
 subsection {* Inequalities on rationals *}
 
@@ -52,6 +57,7 @@ setup {* add_backward_prfstep @{thm positive_imp_inverse_positive} *}
 setup {* add_backward2_prfstep @{thm add_strict_mono} *}
 setup {* add_backward2_prfstep @{thm add_pos_pos} *}
 setup {* add_backward2_prfstep @{thm mult_pos_pos} *}
+setup {* add_backward2_prfstep @{thm divide_pos_pos} *}
 theorem mult_strict_mono' [forward]:
   "(b::('a::linordered_field)) * d \<le> a * c \<Longrightarrow> a < b \<Longrightarrow> 0 < b \<Longrightarrow> 0 \<le> c \<Longrightarrow> c \<ge> d"
   by (meson leD leI mult_strict_mono)
@@ -59,8 +65,10 @@ setup {* add_backward2_prfstep @{thm less_imp_inverse_less} *}
 setup {* add_resolve_prfstep @{thm le_of_int_ceiling} *}
 theorem two_power_gt_zero: "2 ^ k > (0::('a::linordered_field))" by simp
 setup {* add_forward_prfstep_cond @{thm two_power_gt_zero} [with_term "(2::(?'a::linordered_field)) ^ ?k"] *}
-setup {* add_forward_prfstep (equiv_forward_th @{thm pos_le_divide_eq}) *}
-setup {* add_forward_prfstep (equiv_forward_th @{thm pos_divide_less_eq}) *}
+theorem pos_le_divide_eq' [forward]: "(a::('a::linordered_field)) \<le> b / c \<Longrightarrow> c > 0 \<longrightarrow> a * c \<le> b"
+  using pos_le_divide_eq by blast
+theorem pos_divide_less_eq' [forward]: "(a::('a::linordered_field)) > b / c \<Longrightarrow> c > 0 \<longrightarrow> a * c > b"
+  using pos_divide_less_eq by blast
 theorem mult_left_less_imp_less' [forward]:
   "(a::('a::linordered_field)) * b < a * c \<Longrightarrow> a > 0 \<Longrightarrow> b < c" by simp
 
@@ -90,7 +98,7 @@ subsection {* Induction and case check on int, rat *}
 
 theorem int_diff_cases' [resolve]: "\<exists>m n. z = int m - int n" using int_diff_cases by blast
 
-theorem rat_cases [resolve]: "\<exists>a b. b > 0 \<and> r = Fract a b" by (induct r) auto
+theorem rat_cases [resolve]: "\<exists>b a. b > 0 \<and> r = Fract a b" by (induct r) auto
 
 subsection {* Archimedean fields *}
 
