Arith_Thms.thy
@@ -4,8 +4,6 @@ theory Arith_Thms
 imports Auto2_Base Order_Thms Logic_Thms Binomial
 begin
 
-setup {* fold add_rew_const [@{term "0::nat"}, @{term "1::nat"}] *}
-
 (* Reducing inequality on natural numbers. *)
 theorem reduce_le_plus_consts: "(x::nat) + n1 \<le> y + n2 \<Longrightarrow> x \<le> y + (n2-n1)" by simp
 theorem reduce_le_plus_consts': "n1 \<ge> n2 \<Longrightarrow> (x::nat) + n1 \<le> y + n2 \<Longrightarrow> x + (n1-n2) \<le> y" by simp
@@ -50,24 +48,51 @@ theorem cv_const6: "(x::nat) \<le> y + n \<Longrightarrow> x \<le> 0 + (y+n)" by
 theorem nat_eq_to_ineqs: "(x::nat) = y + n \<Longrightarrow> x \<le> y + n \<and> x \<ge> y + n" by simp
 theorem nat_ineq_impl_not_eq: "(x::nat) + n \<le> y \<Longrightarrow> n > 0 \<Longrightarrow> x \<noteq> y" by simp
 
+(* AC-property of +, *, gcd. *)
+theorem add_is_assoc: "is_assoc_fn (op +::'a::semigroup_add \<Rightarrow> 'a \<Rightarrow> 'a)" by (simp add: add.semigroup_axioms is_assoc_fn_def semigroup.assoc)
+theorem add_is_comm: "is_comm_fn (op +::'a::ab_semigroup_add \<Rightarrow> 'a \<Rightarrow> 'a)" by (simp add: add.commute is_comm_fn_def)
+theorem add_has_unit: "is_unit_fn (0::'a::monoid_add) (op +)" by (simp add: is_unit_fn_def)
+theorem add_has_uinv: "is_uinv_fn (op +) (0::'a::ab_group_add) uminus" by (simp add: is_uinv_fn_def)
+theorem add_has_inv: "is_inv_fn (op +::'a::group_add \<Rightarrow> 'a \<Rightarrow> 'a) uminus (op -)" by (simp add: is_inv_fn_def)
+
+theorem mult_is_assoc: "is_assoc_fn (op *::'a::semigroup_mult \<Rightarrow> 'a \<Rightarrow> 'a)" by (simp add: mult.semigroup_axioms is_assoc_fn_def semigroup.assoc)
+theorem mult_is_comm: "is_comm_fn (op *::'a::ab_semigroup_mult \<Rightarrow> 'a \<Rightarrow> 'a)" by (simp add: mult.commute is_comm_fn_def)
+theorem mult_has_unit: "is_unit_fn (1::'a::monoid_mult) (op *)" by (simp add: is_unit_fn_def)
+theorem mult_has_uinv: "is_uinv_fn (op *) (1::'a::field) inverse" by (simp add: is_uinv_fn_def)
+theorem mult_has_inv: "is_inv_fn (op *::'a::field \<Rightarrow> 'a \<Rightarrow> 'a) inverse (op /)" by (simp add: field_class.field_divide_inverse is_inv_fn_def)
+
+theorem gcd_is_assoc: "is_assoc_fn (gcd::nat \<Rightarrow> nat \<Rightarrow> nat)" by (simp add: gcd.semigroup_axioms is_assoc_fn_def semigroup.assoc)
+theorem gcd_is_comm: "is_comm_fn (gcd::nat \<Rightarrow> nat \<Rightarrow> nat)" using gcd_commute_nat is_comm_fn_def by blast
+theorem gcd_has_unit: "is_unit_fn (0::nat) gcd" by (simp add: is_unit_fn_def)
+
 ML_file "arith.ML"
 ML_file "order.ML"
 
 (* General rings. *)
-theorem divide_cancel [rewrite]: "(a::('a::field)) \<noteq> 0 \<Longrightarrow> bu * a * inverse a = bu" by simp
-setup {* add_rewrite_rule_back_cond @{thm ring_distribs(2)} [with_filt (order_filter "a" "b")] *}
-setup {* add_rewrite_rule_back @{thm left_diff_distrib} *}
+theorem double_neg [rewrite]: "(a::('a::ring)) = -b \<Longrightarrow> -a = b" by simp
+theorem divide_cancel [rewrite]: "(a::('a::field)) \<noteq> 0 \<Longrightarrow> a * inverse a * bu = bu" by simp
+theorem ring_distrib: "((a::('a::{semiring,one})) + b) * c = a * c + b * c" by (simp add: ring_distribs)
+setup {* add_rewrite_rule_back_cond @{thm ring_distrib}
+  [with_cond "?c \<noteq> 1", with_filt (order_filter "a" "b")] *}
+theorem ring_distrib_minus: "((a::('a::{ring,one})) - b) * c = a * c - b * c" by (simp add: left_diff_distrib)
+setup {* add_rewrite_rule_back_cond @{thm ring_distrib_minus} [with_cond "?c \<noteq> 1"] *}
 
 ML_file "rings.ML"
 ML_file "rings_test.ML"
+
+(* Property predicates on numbers. *)
+definition is_positive :: "'a::{ord,zero} \<Rightarrow> bool" where
+  "is_positive x \<longleftrightarrow> (x > 0)"
+definition is_negative :: "'a::{ord,zero} \<Rightarrow> bool" where
+  "is_negative x \<longleftrightarrow> (x < 0)"
+setup {* fold add_property_const [@{term "is_positive"}, @{term "is_negative"}] *}
 
 (* Ordering on Nats. *)
 theorem lt_one: "(m::nat) < 1 \<Longrightarrow> m = 0" by simp
 setup {* add_forward_prfstep_cond @{thm lt_one} [with_cond "?m \<noteq> 0"] *}
 setup {* add_resolve_prfstep @{thm Nat.le0} *}
-setup {* add_backward_prfstep_cond @{thm Nat.mult_le_mono1} [with_cond "?k \<noteq> 1"] *}
-setup {* add_resolve_prfstep @{thm Nat.trans_le_add2} *}
-setup {* add_resolve_prfstep_cond @{thm Nat.not_add_less1} [with_filt (not_numc_filter "j")] *}
+setup {* add_backward_prfstep_cond @{thm Nat.mult_le_mono1} [with_term "?k", with_cond "?k \<noteq> 1"] *}
+setup {* add_resolve_prfstep_cond @{thm Nat.not_add_less1} [with_term "?i", with_filt (not_numc_filter "j")] *}
 theorem not_minus_less: "\<not>(i::nat) < (i - j)" by simp
 setup {* add_resolve_prfstep_cond @{thm not_minus_less} [with_filt (not_numc_filter "j")] *}
 
@@ -78,7 +103,7 @@ setup {* add_forward_prfstep_cond @{thm nat_less_diff_conv} [with_filt (not_numc
 theorem Nat_le_diff_conv2_same [forward]: "(i::nat) \<le> i - j \<Longrightarrow> j \<le> i \<Longrightarrow> j = 0" by simp
 theorem Nat_le_diff1_conv [forward]: "(n::nat) \<le> n - 1 \<Longrightarrow> n = 0" by simp
 theorem nat_gt_zero [forward]: "b - a > 0 \<Longrightarrow> b > (a::nat)" by simp
-theorem Nat_le_add_diff_inverse [rewrite]: "(b::nat) \<le> a \<Longrightarrow> b + (a - b) = a" by simp
+setup {* add_rewrite_rule @{thm le_add_diff_inverse} *}
 setup {* add_rewrite_rule @{thm Nat.diff_diff_cancel} *}
 
 (* Intervals. *)
@@ -87,7 +112,8 @@ definition closed_interval :: "nat \<Rightarrow> nat \<Rightarrow> nat \<Rightar
 setup {* fold add_rewrite_rule [@{thm open_interval_def}, @{thm closed_interval_def}] *}
 
 (* Addition. *)
-setup {* add_forward_prfstep @{thm Nat.add_eq_self_zero} *}
+theorem nat_add_eq_self_zero': "(m::nat) = m + n \<Longrightarrow> n = 0" by simp
+setup {* add_forward_prfstep @{thm nat_add_eq_self_zero'} *}
 theorem nat_mult_2: "(a::nat) + a = 2 * a" by simp
 setup {* add_rewrite_rule_cond @{thm nat_mult_2} [with_cond "?a \<noteq> 0"] *}
 
@@ -95,6 +121,7 @@ setup {* add_rewrite_rule_cond @{thm nat_mult_2} [with_cond "?a \<noteq> 0"] *}
 setup {* add_rewrite_rule @{thm Nat.minus_nat.diff_0} *}
 setup {* add_rewrite_rule @{thm Nat.diff_self_eq_0} *}
 setup {* add_rewrite_rule @{thm Nat.diff_add_inverse} *}
+setup {* add_rewrite_rule @{thm Nat.diff_add_inverse2} *}
 theorem n_minus_1_eq_0 [forward]: "(n::nat) \<noteq> 0 \<Longrightarrow> n - 1 = 0 \<Longrightarrow> n = 1" by simp
 theorem diff_distrib: "(i::nat) \<le> k \<Longrightarrow> k \<le> j \<Longrightarrow> j - (k - i) = j - k + i" by simp
 setup {* add_rewrite_rule_cond @{thm diff_distrib} (with_filts [size1_filter "j", size1_filter "k", size1_filter "i"]) *}
@@ -105,6 +132,8 @@ theorem diff_eq_zero' [forward]: "j - k + i = j \<Longrightarrow> (k::nat) \<le>
 
 (* Divides. *)
 setup {* add_forward_prfstep_cond (equiv_forward_th @{thm dvd_def}) (with_conds ["?a \<noteq> ?b", "?a \<noteq> ?b * ?k"]) *}
+setup {* add_gen_prfstep ("shadow_exists_triv",
+  [WithFact @{term_pat "\<exists>x. (?a::nat) = ?a * x"}, ShadowFirst]) *}
 setup {* add_forward_prfstep_cond @{thm Nat.dvd.order.trans}
   (with_conds ["?a \<noteq> ?b", "?b \<noteq> ?c", "?a \<noteq> ?c"]) *}
 setup {* add_forward_prfstep_cond @{thm Nat.dvd.antisym} [with_cond "?x \<noteq> ?y"] *}
@@ -114,9 +143,6 @@ setup {* add_forward_prfstep (equiv_forward_th @{thm dvd_add_right_iff}) *}
 (* Divisibility: existence. *)
 setup {* add_resolve_prfstep @{thm dvd_refl} *}
 theorem exists_n_dvd_n [backward]: "P (n::nat) \<Longrightarrow> \<exists>k. k dvd n \<and> P k" using dvd_refl by blast
-theorem exists_dvd_prod: "\<forall>m::nat. m dvd a * b \<longrightarrow> P m \<Longrightarrow> P a" using dvd_triv_left by blast
-setup {* add_forward_prfstep_cond @{thm exists_dvd_prod}
-  (with_filt (ac_atomic_filter @{const_name times} "a") :: with_conds ["?a \<noteq> 1", "?b \<noteq> 1"]) *}
 setup {* add_resolve_prfstep @{thm one_dvd} *}
 
 theorem any_n_dvd_0 [forward]: "\<not> (\<exists> k. k dvd (0::nat) \<and> P k) \<Longrightarrow> \<not> (\<exists> k. P k)" by simp
@@ -126,18 +152,15 @@ setup {* add_forward_prfstep_cond @{thm n_dvd_one} [with_cond "?n \<noteq> 1"] *
 
 (* Products. *)
 setup {* add_rewrite_rule @{thm mult_zero_left} *}
-theorem prod_ineqs: "(n::nat) = m * k \<Longrightarrow> n > 0 \<Longrightarrow> 1 \<le> m \<and> m \<le> n" by simp
+theorem prod_ineqs: "(n::nat) = m * k \<Longrightarrow> n > 0 \<Longrightarrow> 1 \<le> m \<and> m \<le> n \<and> 1 \<le> k \<and> k \<le> n" by simp
 setup {* add_forward_prfstep_cond @{thm prod_ineqs}
-  ([with_filt (ac_atomic_filter @{const_name times} "m"),
-    with_filt (size1_filter "n")] @
-   (with_conds ["?m \<noteq> 1", "?k \<noteq> 1", "?n \<noteq> ?m", "?n \<noteq> ?k"])) *}
+  (with_filt (size1_filter "n") :: with_conds ["?m \<noteq> 1", "?k \<noteq> 1", "?n \<noteq> ?m", "?n \<noteq> ?k"]) *}
 setup {* add_prfstep_custom
   ("prod_ineqs'",
    [WithFact @{term_pat "(?NUMC::nat) = ?m * ?k"},
     Filter (fn _ => fn (_, inst) => Nat_Arith.lookup_numc0 inst >= 2),
-    Filter (ac_atomic_filter @{const_name times} "m"),
     Filter (not_numc_filter "m")],
-   [Update.ADD_ITEMS],
+   PRIORITY_ADD,
    (fn ((id, inst), ths) => fn _ => fn _ =>
        [Update.thm_update (id, [the_single ths, Nat_Arith.nat_less_th 0 (Nat_Arith.lookup_numc0 inst)] MRS @{thm prod_ineqs})])) *}
 
@@ -149,12 +172,12 @@ setup {* add_forward_prfstep_cond @{thm mult_n1n} [with_cond "?m \<noteq> 1"] *}
 
 theorem prod_is_one [forward]: "(x::nat) * y = 1 \<Longrightarrow> x = 1" by simp
 
-theorem prod_dvd_intro: "(k::nat) dvd m \<or> k dvd n \<Longrightarrow> k dvd m * n" using dvd_mult dvd_mult2 by blast
-setup {* add_backward_prfstep_cond @{thm prod_dvd_intro}
-  [with_filt (canonical_split_filter @{const_name times} "m" "n")] *}
+theorem prod_dvd_intro [backward]: "(k::nat) dvd m \<or> k dvd n \<Longrightarrow> k dvd m * n"
+  using dvd_mult dvd_mult2 by blast
 
 (* Definition of gcd. *)
 setup {* add_forward_prfstep_cond @{thm gcd_dvd1_nat} [with_term "gcd ?a ?b"] *}
+setup {* add_forward_prfstep_cond @{thm gcd_dvd2_nat} [with_term "gcd ?a ?b"] *}
 
 (* Coprimality. *)
 setup {* add_backward_prfstep @{thm coprime_exp_nat} *}
