Auto2_Test.thy
@@ -14,5 +14,6 @@ ML_file "acdata_test.ML"
 ML_file "subterms_test.ML"
 ML_file "normalize_test.ML"
 ML_file "rewrite_test.ML"
+ML_file "matcher_test.ML"
 
 end
