Set_Thms.thy
@@ -8,32 +8,29 @@ section {* Set *}
 
 subsection {* AC property of intersection and union *}
 
+theorem Int_is_assoc: "is_assoc_fn (op \<inter>)" by (simp add: inf.semigroup_axioms is_assoc_fn_def semigroup.assoc)
+theorem Int_is_comm: "is_comm_fn (op \<inter>)" by (simp add: inf_commute is_comm_fn_def)
+theorem Int_has_unit: "is_unit_fn UNIV (op \<inter>)" by (simp add: is_unit_fn_def)
+
+theorem Un_is_assoc: "is_assoc_fn (op \<union>)" by (simp add: is_assoc_fn_def semigroup.assoc sup.semigroup_axioms)
+theorem Un_is_comm: "is_comm_fn (op \<union>)" by (simp add: is_comm_fn_def sup_commute)
+theorem Un_has_unit: "is_unit_fn {} (op \<union>)" by (simp add: is_unit_fn_def)
+
 ML {*
 val add_set_ac_data =
   fold ACUtil.add_ac_data [
-    {fname = @{const_name inf}, assoc_r = false,
-     assoc_th = @{thm Int_ac(1)}, comm_th = @{thm Int_ac(3)},
-     unit_val = @{term UNIV}, unit_th = @{thm Set.Int_UNIV_left}, unitr_th = true_th,
-     uinv_name = "", inv_name = "", double_inv_th = true_th,
-     distr_inv_th = true_th, binop_inv_th = true_th, unit_inv_th = true_th},
+    {fname = @{const_name inf},
+     assoc_th = @{thm Int_is_assoc}, comm_th = @{thm Int_is_comm},
+     unit_th = @{thm Int_has_unit}, uinv_th = true_th, inv_th = true_th},
 
-    {fname = @{const_name sup}, assoc_r = false,
-     assoc_th = @{thm Un_ac(1)}, comm_th = @{thm Un_ac(3)},
-     unit_val = @{term "{}"}, unit_th = @{thm Set.Un_empty_left}, unitr_th = true_th,
-     uinv_name = "", inv_name = "", double_inv_th = true_th,
-     distr_inv_th = true_th, binop_inv_th = true_th, unit_inv_th = true_th}]
+    {fname = @{const_name sup},
+     assoc_th = @{thm Un_is_assoc}, comm_th = @{thm Un_is_comm},
+     unit_th = @{thm Un_has_unit}, uinv_th = true_th, inv_th = true_th}]
 *}
 setup {* add_set_ac_data *}
 
 subsection {* Collection and bounded quantification *}
 setup {* add_rewrite_rule @{thm Set.mem_Collect_eq} *}
-setup {* add_forward_prfstep (equiv_forward_th @{thm Ball_def}) *}
-setup {* add_backward_prfstep (equiv_backward_th @{thm Ball_def}) *}
-theorem ball_subset [forward]: "\<forall>x\<in>s. P x \<Longrightarrow> t \<subseteq> s \<Longrightarrow> \<forall>x\<in>t. P x" by auto
-setup {* add_forward_prfstep_cond (equiv_forward_th @{thm Set.ball_Un})
-  [with_filt (canonical_split_filter @{const_name sup} "A" "B")] *}
-theorem set_ball_Un_backward [forward]: "\<forall>x\<in>A. P x \<Longrightarrow> \<not>(\<forall>x\<in>A\<union>B. P x) \<Longrightarrow> \<not>(\<forall>x\<in>B. P x)" by auto
-setup {* add_rewrite_rule @{thm Set.ball_empty} *}
 theorem ball_single [rewrite]: "(\<forall>x\<in>{x}. P x) = P x" by auto
 
 subsection {* Membership *}
@@ -46,14 +43,13 @@ theorem non_univ_exist_compl [backward]: "U \<noteq> UNIV \<Longrightarrow> \<ex
 theorem univ_member_all [resolve]: "U = UNIV \<Longrightarrow> x \<in> U" by simp
 
 subsection {* Union *}
-theorem set_not_in_union: "x \<notin> A \<union> B \<Longrightarrow> x \<notin> A \<and> x \<notin> B" by auto
-setup {* add_forward_prfstep_cond @{thm set_not_in_union}
-  [with_filt (canonical_split_filter @{const_name sup} "A" "B")] *}
+theorem set_not_in_union [forward]: "x \<notin> A \<union> B \<Longrightarrow> x \<notin> A \<and> x \<notin> B" by auto
 theorem set_in_union_mp: "x \<in> A \<union> B \<Longrightarrow> x \<notin> A \<Longrightarrow> x \<in> B" by auto
 setup {* add_forward_prfstep_cond @{thm set_in_union_mp} [with_cond "?A \<noteq> {?y}"] *}
 theorem set_in_union_mp_single [forward]: "x \<in> {y} \<union> B \<Longrightarrow> x \<noteq> y \<Longrightarrow> x \<in> B" by auto
 theorem union_single_eq [rewrite, backward]: "x \<in> p \<Longrightarrow> {x} \<union> p = p" by auto
-theorem set_eq_union_same [backward]: "A = B \<Longrightarrow> C \<union> A = C \<union> B" by simp
+setup {* add_prfstep (AC_ProofSteps.ac_equiv_strong (
+  "ac_equiv_strong_union", @{term_pat "?A \<union> ?B \<noteq> ?C \<union> ?D"})) *}
 
 subsection {* Disjointness *}
 theorem set_disjoint_mp: "A \<inter> B = {} \<Longrightarrow> p \<in> A \<Longrightarrow> p \<notin> B" by auto
@@ -66,11 +62,13 @@ theorem subset_single [rewrite]: "{a} \<subseteq> B \<longleftrightarrow> a \<in
 setup {* add_forward_prfstep @{thm set_mp} *}
 setup {* add_resolve_prfstep @{thm Set.basic_monos(1)} *}
 setup {* add_resolve_prfstep @{thm Set.Un_upper1} *}
-theorem subset_union_same [backward]: "B \<subseteq> C \<Longrightarrow> A \<union> B \<subseteq> A \<union> C" by auto
+theorem subset_union_same: "B \<subseteq> C \<Longrightarrow> A \<union> B \<subseteq> A \<union> C" by auto
+setup {* add_backward_prfstep_cond @{thm subset_union_same} [with_term "?A"] *}
 
 subsection {* Diff *}
 setup {* add_rewrite_rule @{thm Set.empty_Diff} *}
 theorem set_union_minus_same [rewrite]: "(A \<union> B) - B = A - B" by auto
+theorem set_union_minus_same' [rewrite]: "(B \<union> A) - B = A - B" by auto
 theorem set_union_minus_distinct [rewrite]: "a \<noteq> c \<Longrightarrow> {a} \<union> (B - {c}) = {a} \<union> B - {c}" by auto
 setup {* add_forward_prfstep_cond @{thm Set.Diff_subset} [with_term "?A - ?B"] *}
 theorem union_subtract_elt [rewrite]: "x \<notin> B \<Longrightarrow> (B \<union> {x}) - {x} = B" by simp
@@ -79,8 +77,7 @@ theorem subset_sub1 [backward]: "x \<in> A \<Longrightarrow> A - {x} \<subset> A
 subsection {* Results on finite sets *}
 setup {* add_resolve_prfstep @{thm Finite_Set.finite.emptyI} *}
 theorem set_finite_single [resolve]: "finite {x}" by simp
-setup {* add_rewrite_rule_cond @{thm Finite_Set.finite_Un}
-  [with_filt (canonical_split_filter @{const_name sup} "F" "G")] *}
+setup {* add_rewrite_rule @{thm Finite_Set.finite_Un} *}
 setup {* add_resolve_prfstep @{thm List.finite_set} *}
 theorem Min_eqI' [backward1]: "finite A \<and> (\<forall>y\<in>A. y \<ge> x) \<Longrightarrow> x \<in> A \<Longrightarrow> Min A = x" using Min_eqI by auto
 theorem Max_ge' [forward]: "finite A \<Longrightarrow> x > Max A \<Longrightarrow> \<not>(x \<in> A)" using Max_ge leD by auto
@@ -128,7 +125,7 @@ setup {* add_forward_prfstep_cond @{thm multi_contain_add_self} [with_term "?A +
 theorem multi_add_right [resolve]: "M \<subseteq># N \<Longrightarrow> M + {#x#} \<subseteq># N + {#x#}" by simp
 theorem multi_Ball_mono' [forward]:
   "M \<subset># N \<Longrightarrow> \<forall>x\<in>set_mset N. P x \<Longrightarrow> \<forall>x\<in>set_mset M. P x" by (meson mem_set_mset_iff mset_lessD)
-setup {* add_rewrite_rule @{thm ball_set_mset_iff} *}
+setup {* add_forward_prfstep (equiv_forward_th @{thm ball_set_mset_iff}) *}
 
 subsection {* swap *}
 setup {* add_backward2_prfstep @{thm mset_swap} *}
